Work in progress

isabelle-thys/Basic_Rules.thy
@@ -25,10 +25,376 @@ lemma assign1_rule:
   shows "qrhl A [assign x e] [] B"
   by (cheat assign1_rule)
 
+lemma substitution1_variable_index_flip: "substitution1_variable (index_flip_substitute1 s) = 
+  index_flip_var_raw (substitution1_variable s)"
+  apply transfer by auto
+
+lemma index_flip_var_raw_substitution1_footprint: "index_flip_var_raw ` substitution1_footprint s =
+  substitution1_footprint (index_flip_substitute1 s)"
+  sorry
+
+lemma index_flip_substitute1_twice[simp]: "index_flip_substitute1 (index_flip_substitute1 s) = s"
+  apply transfer by (auto simp: image_iff)
+
+lemma Ex_substitute: "(\<exists>s. P s) \<longleftrightarrow> (\<exists>s. P (f s))" if "surj f" for f::"'x\<Rightarrow>'y" and P
+  using that by (metis UNIV_I bex_imageD)
+
+lemma map_option_Some_eq: "map_option f e = Some (f y) \<longleftrightarrow> e = Some y" if "inj f"
+  by (simp add: inj_eq that)
+
+lemma tmpREMOVE: "a b c \<Longrightarrow> Transfer.Rel a b c" unfolding Transfer.Rel_def by simp
+
+lemma left_unique_rel_mem2[transfer_rule]: assumes "left_total R" shows "left_unique (rel_mem2 R)"
+proof -
+  have left_unique_fun: "left_unique (rel_fun R ((=)))"
+    apply (rule left_unique_fun)
+    using assms left_unique_eq by auto
+  have "m=m'" if "rel_mem2 R m m2" and "rel_mem2 R m' m2" for m m' m2
+  proof -
+    from that have "rel_fun R (=) (Rep_mem2 m) (Rep_mem2 m2)" by (simp add: rel_mem2.rep_eq)
+    moreover from that have "rel_fun R (=) (Rep_mem2 m') (Rep_mem2 m2)" by (simp add: rel_mem2.rep_eq)
+    ultimately have "Rep_mem2 m = Rep_mem2 m'"
+      by (rule left_unique_fun[unfolded left_unique_def, rule_format])
+    then show "m = m'"
+      using Rep_mem2_inject by auto 
+  qed
+  then show ?thesis
+    by (simp add: left_uniqueI)
+qed
+
+lemma rel_mem2_flip[simp]: "(rel_mem2 x)^--1 = (rel_mem2 x^--1)"
+    apply (rule ext)+ unfolding conversep_iff apply transfer
+    by (auto simp: rel_fun_def)
+
+lemma right_unique_rel_mem2[transfer_rule]: assumes "right_total R" shows "right_unique (rel_mem2 R)"
+  apply (subst conversep_conversep[of R, symmetric])
+  apply (subst rel_mem2_flip[symmetric])
+  apply (simp del: rel_mem2_flip)
+  apply (rule left_unique_rel_mem2)
+  using assms by simp
+
+lemma bi_unique_rel_mem2[transfer_rule]: assumes "bi_total R" shows "bi_unique (rel_mem2 R)"
+  using assms bi_total_alt_def bi_unique_alt_def left_unique_rel_mem2 right_unique_rel_mem2 by blast
+
+definition "type_preserving_var_rel R \<longleftrightarrow> (\<forall>v w. R v w \<longrightarrow> variable_raw_domain v = variable_raw_domain w)"
+
+lemma left_total_rel_mem2[transfer_rule]: 
+  assumes "left_unique R" and "right_total R" and "type_preserving_var_rel R"
+  shows "left_total (rel_mem2 R)"
+proof -
+  have "\<exists>m2. rel_mem2 R m1 m2" for m1
+  proof (transfer fixing: R, auto)
+    fix m1 
+    assume m1v: "\<forall>v. m1 v \<in> variable_raw_domain v"
+    have left_total_fun: "left_total (rel_fun R (=))"
+      apply (rule left_total_fun)
+      using \<open>left_unique R\<close> by (auto simp: left_total_eq)
+    then obtain m2 where m2: "rel_fun R (=) m1 m2" 
+      using left_totalE by auto
+    have m2v: "m2 v \<in> variable_raw_domain v" for v
+    proof -
+      obtain w where "R w v"
+        apply atomize_elim using \<open>right_total R\<close> unfolding right_total_def by simp
+      with m2 have m1m2: "m1 w = m2 v"
+        by (rule rel_funD)
+      from \<open>R w v\<close> \<open>type_preserving_var_rel R\<close> have "variable_raw_domain v = variable_raw_domain w"
+        unfolding type_preserving_var_rel_def by simp
+      with m1v[rule_format, of w] m1m2 
+      show ?thesis by auto
+    qed
+    from m2 m2v 
+    show "\<exists>x. (\<forall>v. x v \<in> variable_raw_domain v) \<and> rel_fun R (=) m1 x"
+      by auto
+  qed
+  then show ?thesis
+    by (rule left_totalI)
+qed
+
+lemma type_preserving_var_rel_flip[simp]: "type_preserving_var_rel R\<inverse>\<inverse> \<longleftrightarrow> type_preserving_var_rel R"
+  unfolding type_preserving_var_rel_def by auto
+
+lemma right_total_rel_mem2[transfer_rule]: 
+  assumes "right_unique R" and "left_total R" and "type_preserving_var_rel R"
+  shows "right_total (rel_mem2 R)"
+  apply (subst conversep_conversep[of R, symmetric])
+  apply (subst rel_mem2_flip[symmetric])
+  apply (simp del: rel_mem2_flip)
+  apply (rule left_total_rel_mem2)
+  using assms by auto
+
+lemma bi_total_rel_mem2[transfer_rule]: 
+  assumes "bi_unique R" and "bi_total R" and "type_preserving_var_rel R"
+  shows "bi_total (rel_mem2 R)"
+  by (meson assms bi_total_alt_def bi_unique_alt_def left_total_rel_mem2 right_total_rel_mem2)
+
+
+lemma left_unique_rel_expression[transfer_rule]:
+  assumes "left_unique R" and "left_unique S" and "right_total R" and "type_preserving_var_rel R"
+  shows "left_unique (rel_expression R S)"
+proof -
+  have "e = f" if "rel_expression R S e g" and "rel_expression R S f g" for e f g
+  proof -
+    obtain vse E where e: "Rep_expression e = (vse,E)" by (atomize_elim, auto)
+    obtain vsf F where f: "Rep_expression f = (vsf,F)" by (atomize_elim, auto)
+    obtain vsg G where g: "Rep_expression g = (vsg,G)" by (atomize_elim, auto)
+    from that have "rel_prod (rel_set R) (rel_fun (rel_mem2 R) S) (vse,E) (vsg,G)"
+      unfolding rel_expression.rep_eq e g by simp
+    then have vseg: "rel_set R vse vsg" and EG: "(rel_fun (rel_mem2 R) S) E G" by auto
+
+    from that have "rel_prod (rel_set R) (rel_fun (rel_mem2 R) S) (vsf,F) (vsg,G)"
+      unfolding rel_expression.rep_eq f g by simp
+    then have vsfg: "rel_set R vsf vsg" and FG: "(rel_fun (rel_mem2 R) S) F G" by auto
+
+    from vseg vsfg have "vse = vsf"
+      using \<open>left_unique R\<close>
+      by (meson left_uniqueD left_unique_rel_set) 
+
+    have left_unique_fun: "left_unique (rel_fun (rel_mem2 R) S)"
+      apply (rule left_unique_fun)
+       apply (rule left_total_rel_mem2)
+      using assms by auto
+    from EG FG have "E = F"
+      using left_unique_fun
+      by (meson left_uniqueD)
+
+    from \<open>vse = vsf\<close> \<open>E = F\<close>
+    show "e = f"
+      using Rep_expression_inject e f by fastforce
+    qed
+  then show ?thesis
+    unfolding left_unique_def by simp
+qed
+
+lemma rel_expression_flip[simp]: "(rel_expression R S)^--1 = rel_expression R^--1 S^--1"
+  apply (rule ext)+ unfolding conversep_iff apply transfer
+  using rel_mem2_flip[unfolded conversep_iff]
+  apply (auto simp: rel_fun_def rel_set_def)
+  by (metis (full_types))+
+
+lemma right_unique_rel_expression[transfer_rule]:
+  assumes "right_unique R" and "right_unique S" and "left_total R" and "type_preserving_var_rel R"
+  shows "right_unique (rel_expression R S)"
+  apply (subst conversep_conversep[of R, symmetric])
+  apply (subst conversep_conversep[of S, symmetric])
+  apply (subst rel_expression_flip[symmetric])
+  apply (simp del: rel_expression_flip)
+  apply (rule left_unique_rel_expression)
+  using assms by auto
+
+lemma bi_unique_rel_expression[transfer_rule]:
+  assumes "bi_unique R" and "bi_unique S" and "bi_total R" and "type_preserving_var_rel R"
+  shows "bi_unique (rel_expression R S)"
+  using assms by (meson bi_total_alt_def bi_unique_alt_def left_unique_rel_expression right_unique_rel_expression)
+
+lemma rel_expression_subst_expression [transfer_rule]: 
+  includes lifting_syntax
+  assumes "bi_unique R" and "bi_total R" and "type_preserving_var_rel R" (* TODO cleanup *)
+  defines "subR == rel_substitute1 R (rel_expression R (=))"
+  shows "(list_all2 subR ===> rel_expression R (=) ===> rel_expression R (=)) 
+         subst_expression subst_expression"
+proof -
+  have "rel_expression R (=) (subst_expression s1 e1) (subst_expression s2 e2)" 
+    if "list_all2 subR s1 s2" and "rel_expression R (=) e1 e2" for s1 s2 and e1 e2 :: "'b expression"
+  proof -
+    obtain vs1 E1 where e1: "Rep_expression e1 = (vs1,E1)" apply atomize_elim by auto
+    obtain vs2 E2 where e2: "Rep_expression e2 = (vs2,E2)" apply atomize_elim by auto
+    have foot: "rel_set R (subst_expression_footprint s1 vs1) (subst_expression_footprint s2 vs2)"
+      apply (rule rel_setI)
+      unfolding subst_expression_footprint_def 
+      apply auto
+      sorry
+    have subst: "(rel_mem2 R ===> (=)) (E1 \<circ> subst_mem2 s1) (E2 \<circ> subst_mem2 s2)" 
+      sorry
+    show ?thesis
+      unfolding rel_expression.rep_eq subst_expression.rep_eq e1 e2 using foot subst by auto
+  qed
+
+  then show ?thesis
+     unfolding subR_def
+    apply (rule_tac rel_funI)+ by assumption
+qed
+
 (* TODO move *)
 lemma index_flip_subst_expression: "index_flip_expression (subst_expression \<sigma> e) 
   = subst_expression (map index_flip_substitute1 \<sigma>) (index_flip_expression e)"
-  by (cheat index_flip_subst_expression)
+proof -
+  define varR where "varR x y \<longleftrightarrow> index_flip_var_raw x = y" for x y
+  have varR_def': "varR x y \<longleftrightarrow> x = index_flip_var_raw y" for x y
+    unfolding varR_def by auto
+  define subR where "subR = (rel_substitute1 varR (rel_expression varR ((=)::'b::universe\<Rightarrow>'b\<Rightarrow>bool)))" 
+    (* for T :: "'b::universe itself" *)
+  (* define expR where "expR x y \<longleftrightarrow> index_flip_expression x = y" for x y :: "'a expression" *)
+  (* let ?expR = "rel_expression varR (=)" *)
+  (* define sub1R where "sub1R x y \<longleftrightarrow> index_flip_substitute1 x = y" for x y *)
+  (* let ?subR = "rel_substitute1 varR (=)" *)
+  have rel_set_varR: "rel_set varR x y \<longleftrightarrow> index_flip_var_raw ` x = y" for x y
+    unfolding rel_set_def varR_def by auto
+
+  include lifting_syntax
+  have [transfer_rule]: "bi_unique varR" 
+    apply (rule bi_uniqueI)
+     apply (rule left_uniqueI, unfold varR_def', auto)[1]
+    by (rule right_uniqueI, unfold varR_def, auto)[1]
+
+  have [transfer_rule]: "bi_total varR"
+    apply (rule bi_totalI)
+     apply (rule left_totalI, unfold varR_def, auto)[1]
+    by (rule right_totalI, unfold varR_def', auto)[1]
+
+  have [transfer_rule]: "type_preserving_var_rel varR"
+    unfolding type_preserving_var_rel_def varR_def by auto 
+
+  have rel_fun_flip[simp]: "(rel_fun x y)^--1 = (rel_fun x^--1 y^--1)" for x :: "'c\<Rightarrow>'d\<Rightarrow>bool" and y :: "'e\<Rightarrow>'f\<Rightarrow>bool" 
+    unfolding rel_fun_def by auto
+(*   have rel_mem2_flip[simp]: "(rel_mem2 x)^--1 = (rel_mem2 x^--1)" for x
+    apply (rule ext)+ unfolding conversep_iff apply transfer
+    by (auto simp: rel_fun_def) *)
+  have [simp]: "varR\<inverse>\<inverse> = varR"
+    apply (rule ext)+ unfolding conversep_iff using varR_def varR_def' by auto
+
+  have "rel_expression varR (=) e (index_flip_expression e)" for e :: "'c expression"
+  proof (unfold rel_expression.rep_eq index_flip_expression.rep_eq, cases "Rep_expression e", auto)
+    fix vs f assume "Rep_expression e = (vs,f)"
+    show "rel_set varR vs (index_flip_var_raw ` vs)"
+      by (rule rel_setI, unfold varR_def, auto)
+    show "(rel_mem2 varR ===> (=)) f (\<lambda>m. f (index_flip_mem2 m))"
+      apply (rule conversepD[of "(rel_mem2 varR ===> (=))"])
+      unfolding rel_fun_flip apply simp
+      unfolding rel_fun_def rel_mem2.rep_eq varR_def' apply transfer by auto
+  qed
+  then have [transfer_rule]: "((=) ===> rel_expression varR (=)) (%x. x) index_flip_expression"
+    unfolding rel_fun_def by auto
+
+  have varR_index_flip_var_raw: "varR v (index_flip_var_raw v)" for v
+    by (simp add: varR_def)
+  have rel_set_varR_index_flip_var_raw: "rel_set varR vs (index_flip_var_raw ` vs)" for vs
+    by (subst rel_set_varR, rule)
+  have "F x = (F \<circ> index_flip_mem2) y" if "rel_mem2 varR x y" for F::"mem2\<Rightarrow>'c" and x y
+    using that apply transfer apply (auto simp: varR_def[abs_def])
+    by (metis (full_types) rel_fun_def)
+  then have inv_embedding_index_flip_mem2: "(rel_mem2 varR ===> (=)) (inv embedding \<circ> f) (inv embedding \<circ> (f \<circ> index_flip_mem2))" for f
+    apply (rule_tac rel_funI) by simp
+
+  have 1: "rel_prod varR
+          (\<lambda>(vs1, f1) (vs2, f2). rel_prod (rel_set varR) (rel_mem2 varR ===> (=)) (vs1, inv embedding \<circ> f1) (vs2, inv embedding \<circ> f2))
+          (v, vs, f) (index_flip_var_raw v, index_flip_var_raw ` vs, f \<circ> index_flip_mem2)" for v vs f
+    by (auto intro: varR_index_flip_var_raw rel_set_varR_index_flip_var_raw inv_embedding_index_flip_mem2)
+
+  have "rel_substitute1 varR (rel_expression varR (=)) s (index_flip_substitute1 s)" for s
+    apply transfer apply (case_tac s) using 1 by simp
+  then have index_flip_substitute1_transfer [transfer_rule]: 
+    "((=) ===> subR) (%x. x) index_flip_substitute1"
+    unfolding subR_def rel_fun_def by auto
+(*   have [transfer_rule]: "bi_unique (rel_expression varR (=))"
+    sorry *)
+  have "index_flip_expression e = f" if that[transfer_rule]: "rel_expression varR (=) e f" for e f :: "'c expression"
+    apply transfer by rule
+  then have [transfer_rule]: "(rel_expression varR (=) ===> rel_expression (=) (=)) index_flip_expression id"
+    apply (rule_tac rel_funI) by (simp add: rel_expression_eq)
+
+(*   have "rel_expression varR (=) (subst_expression s1 e1) (subst_expression s2 e2)" 
+    if "list_all2 subR s1 s2" and "rel_expression varR (=) e1 e2" for s1 s2 e1 e2
+    apply transfer
+    sorry *)
+
+(*  then have [transfer_rule]:
+    "(list_all2 subR ===> rel_expression varR (=) ===> rel_expression varR (=)) 
+    subst_expression subst_expression"
+     unfolding subR_def
+    apply (rule_tac rel_funI)+ by assumption *)
+
+  note rel_expression_subst_expression[where R=varR, folded subR_def, transfer_rule]
+
+  have "(rel_expression (=) (=))
+        (index_flip_expression (subst_expression \<sigma> e))
+        (id (subst_expression (map index_flip_substitute1 \<sigma>) (index_flip_expression e)))"
+    apply transfer_prover_start
+           apply transfer_step+
+    by simp
+  then
+  show "index_flip_expression (subst_expression \<sigma> e) = subst_expression (map index_flip_substitute1 \<sigma>) (index_flip_expression e)"
+    unfolding rel_expression_eq id_def by assumption
+qed
+
+(* (* TODO move *)
+lemma index_flip_subst_expression: "index_flip_expression (subst_expression \<sigma> e) 
+  = subst_expression (map index_flip_substitute1 \<sigma>) (index_flip_expression e)"
+proof -
+  have image: "x \<in> index_flip_var_raw ` X \<longleftrightarrow> index_flip_var_raw x \<in> X" for x X
+    by force
+  have uni_split: "A=A' \<Longrightarrow> B=B' \<Longrightarrow> A\<union>B = A'\<union>B'" for A B A' B' :: "'x set" 
+    by auto
+  have UNI_split: "X = Y \<Longrightarrow> \<Union>X = \<Union>Y" for X Y :: "'x set set" by auto
+  have index_flip_substitute1_inj: "inj index_flip_substitute1" sorry
+
+(* IDEA: Use transfer to show the equality, by relating the lhs/rhs via index_flip_var_raw *)
+
+  define vs where "vs = expression_vars e"
+  have "expression_vars (index_flip_expression (subst_expression \<sigma> e)) = 
+        index_flip_var_raw ` subst_expression_footprint \<sigma> vs"
+    by (simp add: subst_expression_footprint vs_def)
+  have "\<dots> = index_flip_var_raw ` Union {substitution1_footprint s | s v. 
+        Some s = find (\<lambda>s. substitution1_variable s = v) \<sigma> \<and> substitution1_variable s \<in> vs}
+        \<union> index_flip_var_raw ` (vs - substitution1_variable ` set \<sigma>)" (is "_ = _ \<union> ?v")
+    unfolding subst_expression_footprint_def by auto
+  have "\<dots>
+      = Union {index_flip_var_raw ` substitution1_footprint s | s v. 
+        Some s = find (\<lambda>s. substitution1_variable s = v) \<sigma> \<and> substitution1_variable s \<in> vs} \<union> ?v" 
+        (is "_ = Union {_ | s v. ?l s v \<and> ?r s v} \<union> _")
+    by auto
+  also have "\<dots> = Union {substitution1_footprint (index_flip_substitute1 s) | s v. ?l s v \<and> ?r s v} \<union> ?v"
+    by (auto simp: index_flip_var_raw_substitution1_footprint)
+  also have "\<dots> = Union {substitution1_footprint (index_flip_substitute1 (index_flip_substitute1 s)) | s v. 
+        Some (index_flip_substitute1 s) = find (\<lambda>s. substitution1_variable s = index_flip_var_raw v) \<sigma> 
+        \<and> substitution1_variable (index_flip_substitute1 s) \<in> vs} \<union> ?v"
+        (is "_ = Union {_ | s v. ?l s v \<and> ?r s v} \<union> _")
+    apply (subst Ex_substitute[where f=index_flip_substitute1])
+    using index_flip_substitute1_twice surjI apply blast 
+    apply (subst Ex_substitute[where f=index_flip_var_raw])
+    using index_flip_var_twice surjI apply blast 
+    by simp
+  also have "\<dots> = Union {substitution1_footprint s | s v. ?l s v \<and> ?r s v} \<union> ?v"
+    by (simp add: substitution1_variable_index_flip) 
+  also have "\<dots> = Union {substitution1_footprint s | s v. 
+         Some s = map_option index_flip_substitute1 (find (\<lambda>s. substitution1_variable s = index_flip_var_raw v) \<sigma>)
+          \<and> ?r s v} \<union> ?v"
+    using map_option_Some_eq[OF index_flip_substitute1_inj] index_flip_substitute1_twice
+    by (metis (no_types, lifting))
+  also have "\<dots> = Union {substitution1_footprint s | s v. 
+         Some s = (find (\<lambda>s. substitution1_variable (index_flip_substitute1 s) = v) (map index_flip_substitute1 \<sigma>))
+          \<and> ?r s v} \<union> ?v"
+      (is "_ = Union {_ | s v. ?l s v \<and> ?r s v} \<union> _")
+    using find_map[where f=index_flip_substitute1 and l=\<sigma>] index_flip_substitute1_twice 
+    apply (subst find_map, auto) by (metis index_flip_var_twice)
+  also have "\<dots> = Union {substitution1_footprint s | s v. 
+         ?l s v \<and> substitution1_variable s \<in> index_flip_var_raw ` vs} \<union> ?v"
+      (is "_ = ?u \<union> ?v")
+    by (simp add: image substitution1_variable_index_flip)
+  also have "\<dots> = ?u \<union> (index_flip_var_raw ` vs - index_flip_var_raw ` substitution1_variable ` set \<sigma>)" 
+
+  also have "\<dots> = subst_expression_footprint (map index_flip_substitute1 \<sigma>) (index_flip_var_raw ` vs)"
+    unfolding subst_expression_footprint_def 
+    apply (unfold image_Un, rule uni_split)
+    apply (subst image, subst find_map)
+    by xxx
+  find_theorems " (_ \<union> _) =  (_ \<union> _)"
+
+  have "expression_vars (subst_expression (map index_flip_substitute1 \<sigma>) (index_flip_expression e))
+      = subst_expression_footprint (map index_flip_substitute1 \<sigma>) (index_flip_var_raw ` vs)"
+    by (simp add: subst_expression_footprint vs_def)
+  have "... = xxx"
+    unfolding subst_expression_footprint_def find_map vimage 
+substitution1_variable_index_flip
+
+  obtain vs E where e: "(vs,E) = Rep_expression e"
+    by (xmetis surj_pair) by auto
+  find_theorems "expression_vars" subst_expression
+  then show ?thesis sorry
+qed
+  apply (subst Rep_expression_inject[symmetric])
+  unfolding index_flip_expression.rep_eq subst_expression.rep_eq
+  apply (cases "Rep_expression e") apply simp
+  by (cheat index_flip_subst_expression) *)
 
 (* TODO move *)
 lemma index_flip_var_index_var_raw[simp]: "index_flip_var_raw (index_var_raw left x) = index_var_raw (\<not> left) x"
